rank golfing

Matroid/Constructions/RankAxioms.lean
@@ -377,89 +377,6 @@ def ofFiniteRankAxioms' (E : Set α) (hE : E.Finite) (r : Set α → ℕ)
       union_eq_self_of_subset_left hAB]
   ofFiniteRankAxioms E r rank_le_ncard monotonicity submodularity rank_inter_ground
 
-def ofFinsetRankAxioms [DecidableEq α] (E : Set α) (r : Finset α → ℕ)
-    (rank_empty : r ∅ = 0)
-    (rank_singleton : ∀ e, r {e} ≤ 1)
-    (submodularity : ∀ A (x y : α), r A + r (A ∪ {x,y}) ≤ r (insert x A) + r (insert y A))
-    (rank_singleton_of_not_mem_ground : ∀ e ∉ E, r {e} = 0) :
-    Matroid α :=
-  have rank_mono : ∀ X Y, r X ≤ r (X ∪ Y) := fun X Y ↦ by
-    induction' Y using Finset.induction with e Y _ hY
-    · simp
-    rw [Finset.union_insert]
-    exact hY.trans (by simpa [Finset.union_comm, Finset.insert_eq] using submodularity (X ∪ Y) e e)
-  have r_insert_le : ∀ {X e}, r (insert e X) ≤ r X + r {e} := fun {X e} ↦ by
-    induction' X using Finset.induction with f X _ hX
-    · simp [rank_empty, rank_singleton e]
-    rw [Finset.insert_eq, Finset.insert_eq, ← Finset.union_assoc, ← Finset.insert_eq,
-      Finset.union_comm, ← X.insert_eq]
-    linarith [submodularity X e f]
-  have r_insert_le' : ∀ {X e}, r (insert e X) ≤ r X + 1 :=
-    fun {X e} ↦ (r_insert_le).trans (add_le_add_left (rank_singleton e) _)
-  have rank_le_card : ∀ X, r X ≤ X.card := fun X ↦ by
-    induction' X using Finset.induction with e X heX hX
-    · simp [rank_empty]
-    rw [Finset.card_insert_of_not_mem (by simpa)]
-    exact r_insert_le'.trans (add_le_add_right hX 1)
-  have indep_empty : r ∅ = (∅ : Finset α).card := le_antisymm (rank_le_card ∅) <| by simp
-  have indep_subset : ∀ I J, r J = J.card → I ⊆ J → r I = I.card := by
-    suffices h' : ∀ I D, (I ∪ D).card ≤ r (I ∪ D) → r I = I.card from
-      fun I J hJ hIJ ↦ h' _ J <| by simpa [Finset.union_eq_right.2 hIJ] using hJ.symm.le
-    intro I D
-    induction' D using Finset.induction with e D heD hD
-    · simp only [Finset.union_empty]
-      exact fun h ↦ h.antisymm' (rank_le_card _)
-    rw [Finset.union_insert]
-    by_cases heI : e ∈ I
-    · rwa [Finset.insert_eq_of_mem (by simp [heI])]
-    refine fun hle ↦ hD ?_
-    replace hle := hle.trans r_insert_le'
-    rwa [Finset.card_insert_of_not_mem (by simp [heI, heD]), add_le_add_iff_right] at hle
-  have indep_aug : ∀ ⦃I J : Finset α⦄, r I = I.card → r J = J.card → I.card < J.card →
-      ∃ e ∈ J, e ∉ I ∧ r (insert e I) = (insert e I).card := by
-    intro I J hI hJ hIJ
-    by_contra! hcon
-    have haux : ∀ S ⊆ J \ I, r (I ∪ S) = r I := fun S ↦ by
-      induction' S using Finset.induction with e S heS ih
-      · simp
-      simp only [Finset.insert_subset_iff, Finset.mem_sdiff, Finset.union_insert, and_imp]
-      intro heJ heI hSJI
-      induction' S using Finset.induction with f S _ ih'
-      · rw [Finset.union_empty, le_antisymm_iff, ← Nat.lt_add_one_iff,
-          hI, ← I.card_insert_of_not_mem heI, lt_iff_le_and_ne, and_iff_right (rank_le_card _),
-          and_iff_right (hcon e heJ heI), ← hI, Finset.insert_eq, Finset.union_comm]
-        apply rank_mono
-      specialize ih hSJI
-      suffices h' : r (I ∪ S ∪ ({e,f})) ≤ r I by
-        rw [Finset.insert_eq, Finset.union_comm, Finset.insert_eq, Finset.union_comm {f},
-          Finset.union_assoc, S.union_assoc, ← Finset.insert_eq, Finset.pair_comm, ← I.union_assoc]
-        exact h'.antisymm (by rw [I.union_assoc]; apply rank_mono)
-      have hsm := submodularity (I ∪ S) e f
-      simp only [Finset.mem_insert, not_or] at heS
-      have hIS : r (I ∪ S) = r I := by
-        rw [← ih, Finset.union_insert, le_antisymm_iff, Finset.insert_eq, Finset.union_comm {f},
-          and_iff_right (rank_mono _ _), Finset.union_assoc, S.union_comm, ← S.insert_eq, ih]
-        apply rank_mono
-      rw [Finset.insert_subset_iff] at hSJI
-      rw [ih' heS.2 (fun _ ↦ hIS) hSJI.2, ← Finset.union_insert, ih, hIS] at hsm
-      linarith
-    have h' : r (J ∪ I) = r I := by simpa [J.union_comm] using haux _ Subset.rfl
-    replace h' := (rank_mono _ _).trans h'.le
-    exact hIJ.not_le <| by rwa [← hI, ← hJ]
-  have indep_support : ∀ ⦃I : Finset α⦄, r I = I.card → (I : Set α) ⊆ E := fun I hI e heI ↦ by
-    by_contra heE
-    have hle := (r_insert_le (X := I.erase e) (e := e)).trans
-      (add_le_add_right (rank_le_card _) _)
-    rw [Finset.insert_erase (by simpa using heI), rank_singleton_of_not_mem_ground e heE,
-      add_zero, hI, ← Finset.card_erase_add_one (by simpa using heI)] at hle
-    simp at hle
-  IndepMatroid.matroid <| IndepMatroid.ofFinset E (fun I ↦ r I = I.card)
-    indep_empty indep_subset indep_aug indep_support
-
-lemma ofFinsetRankAxioms_rank_eq [DecidableEq α] (E : Set α) (r : Finset α → ℕ)
-    (h1) (h2) (h3) (h4) (X : Finset α) :
-    (Matroid.ofFinsetRankAxioms E r h1 h2 h3 h4).r X = r X := by
-  sorry
 
 def ofFinitaryRankAxioms [DecidableEq α] (E : Set α) [DecidablePred (· ∈ E)]
     (r : Finset α → ℕ)
@@ -542,3 +459,159 @@ def ofFinitaryRankAxioms [DecidableEq α] (E : Set α) [DecidablePred (· ∈ E)
     contradiction
   IndepMatroid.matroid <| IndepMatroid.ofFinitary E Indep indep_empty
     indep_subset indep_aug indep_compact subset_ground
+
+end Matroid
+section FinsetRank
+
+structure FinsetRankMatroid (α : Type*) [DecidableEq α] where
+  E : Set α
+  r : Finset α → ℕ
+  r_empty : r ∅ = 0
+  r_singleton : ∀ e, r {e} ≤ 1
+  r_insert_insert : ∀ X e f, r X + r (X ∪ {e,f}) ≤ r (insert e X) + r (insert f X)
+  r_singleton_of_not_mem_ground : ∀ e ∉ E, r {e} = 0
+namespace FinsetRankMatroid
+
+variable {α : Type*} {X Y I J : Finset α} {e f : α} [DecidableEq α] {M : FinsetRankMatroid α}
+
+open Finset
+
+lemma r_le_union : M.r X ≤ M.r (X ∪ Y) := by
+  induction' Y using Finset.induction with e Y _ hY
+  · simp
+  rw [X.union_insert]
+  exact hY.trans (by simpa [Finset.union_comm, Finset.insert_eq]
+    using M.r_insert_insert (X ∪ Y) e e)
+
+lemma r_mono (h : X ⊆ Y) : M.r X ≤ M.r Y := by
+  rw [← Finset.union_eq_right.2 h]
+  apply r_le_union
+
+lemma r_insert_le : M.r (insert e X) ≤ M.r X + M.r {e} := by
+  induction' X using Finset.induction with f X _ hX
+  · simp [r_empty, M.r_singleton e]
+  rw [Finset.insert_eq, Finset.insert_eq, ← Finset.union_assoc, ← Finset.insert_eq,
+    Finset.union_comm, ← X.insert_eq]
+  linarith [M.r_insert_insert X e f]
+
+lemma r_insert_le' : M.r (insert e X) ≤ M.r X + 1 := by
+  refine r_insert_le.trans (add_le_add_left (M.r_singleton e) _)
+
+lemma r_le_card : M.r X ≤ X.card := by
+  induction' X using Finset.induction with e X heX hX
+  · simp [r_empty]
+  rw [Finset.card_insert_of_not_mem (by simpa)]
+  exact r_insert_le'.trans (add_le_add_right hX 1)
+
+lemma indep_empty : M.r ∅ = (∅ : Finset α).card :=
+  le_antisymm M.r_le_card <| by simp
+
+lemma indep_subset (hJ : M.r J = J.card) (hIJ : I ⊆ J) : M.r I = I.card := by
+  suffices h' : ∀ I D : Finset α, (I ∪ D).card ≤ M.r (I ∪ D) → M.r I = I.card from
+      h' _ J <| by simpa [Finset.union_eq_right.2 hIJ] using hJ.symm.le
+  intro I D
+  induction' D using Finset.induction with e D heD hD
+  · simp only [Finset.union_empty]
+    exact fun h ↦ h.antisymm' M.r_le_card
+  rw [Finset.union_insert]
+  by_cases heI : e ∈ I
+  · rwa [Finset.insert_eq_of_mem (by simp [heI])]
+  refine fun hle ↦ hD ?_
+  replace hle := hle.trans r_insert_le'
+  rwa [Finset.card_insert_of_not_mem (by simp [heI, heD]), add_le_add_iff_right] at hle
+
+lemma indep_aug' (hI : M.r I = I.card) (hlt : M.r I < M.r X) :
+    ∃ e ∈ X, e ∉ I ∧ M.r (insert e I) = (insert e I).card := by
+  by_contra! hcon
+  have haux : ∀ S ⊆ X \ I, M.r (I ∪ S) = M.r I := fun S ↦ by
+    induction' S using Finset.induction with e S heS ih
+    · simp
+    simp only [Finset.insert_subset_iff, Finset.mem_sdiff, Finset.union_insert, and_imp]
+    intro heX heI hSJI
+    induction' S using Finset.induction with f S _ ih'
+    · rw [Finset.union_empty, le_antisymm_iff, ← Nat.lt_add_one_iff,
+        hI, ← I.card_insert_of_not_mem heI, lt_iff_le_and_ne, and_iff_right M.r_le_card,
+        and_iff_right (hcon e heX heI), ← hI, Finset.insert_eq, Finset.union_comm]
+      apply M.r_le_union
+    specialize ih hSJI
+    suffices h' : M.r (I ∪ S ∪ ({e,f})) ≤ M.r I by
+      rw [Finset.insert_eq, Finset.union_comm, Finset.insert_eq, Finset.union_comm {f},
+        Finset.union_assoc, S.union_assoc, ← Finset.insert_eq, Finset.pair_comm, ← I.union_assoc]
+      exact h'.antisymm (by rw [I.union_assoc]; apply M.r_le_union)
+    have hsm := M.r_insert_insert (I ∪ S) e f
+    simp only [Finset.mem_insert, not_or] at heS
+    have hIS : M.r (I ∪ S) = M.r I := by
+      rw [← ih, Finset.union_insert, le_antisymm_iff, Finset.insert_eq, Finset.union_comm {f},
+        and_iff_right M.r_le_union, Finset.union_assoc, S.union_comm, ← S.insert_eq, ih]
+      apply M.r_le_union
+    rw [Finset.insert_subset_iff] at hSJI
+    rw [ih' heS.2 (fun _ ↦ hIS) hSJI.2, ← Finset.union_insert, ih, hIS] at hsm
+    linarith
+  have h' : M.r (X ∪ I) = M.r I := by simpa [X.union_comm] using haux _ Finset.Subset.rfl
+  exact hlt.not_le <| le_trans M.r_le_union h'.le
+
+lemma indep_aug (hI : M.r I = I.card) (hJ : M.r J = J.card) (hlt : I.card < J.card) :
+    ∃ e ∈ J, e ∉ I ∧ M.r (insert e I) = (insert e I).card :=
+  indep_aug' hI (by rwa [hI, hJ])
+
+lemma indep_support (hI : M.r I = I.card) : (I : Set α) ⊆ M.E := by
+  refine fun e heI ↦ by_contra fun heE ↦ ?_
+  have hle := (r_insert_le (X := I.erase e) (e := e)).trans
+    (add_le_add_right M.r_le_card _)
+  rw [Finset.insert_erase (by simpa using heI), M.r_singleton_of_not_mem_ground e heE,
+    add_zero, hI, ← Finset.card_erase_add_one (by simpa using heI)] at hle
+  simp at hle
+
+@[simps! E] protected def matroid (M : FinsetRankMatroid α) : Matroid α :=
+   IndepMatroid.matroid <| IndepMatroid.ofFinset M.E (fun I ↦ M.r I = I.card)
+    indep_empty (fun _ _ ↦ indep_subset) (fun _ _ ↦ indep_aug) (fun _ ↦ indep_support)
+
+@[simp] protected lemma matroid_indep_iff {I : Finset α} : M.matroid.Indep I ↔ M.r I = I.card := by
+  simp [FinsetRankMatroid.matroid]
+
+instance : M.matroid.Finitary := by
+  rw [FinsetRankMatroid.matroid, IndepMatroid.ofFinset]
+  infer_instance
+
+protected lemma matroid_indep_iff' {I : Set α} :
+    M.matroid.Indep I ↔ ∀ J : Finset α, (J : Set α) ⊆ I → M.r J = J.card := by
+  simp [FinsetRankMatroid.matroid, IndepMatroid.ofFinset_indep']
+
+@[simp] protected lemma matroid_r_eq (X : Finset α) : M.matroid.r X = M.r X := by
+  obtain ⟨I, hI⟩ := M.matroid.exists_basis' X
+  obtain ⟨I, rfl⟩ := (X.finite_toSet.subset hI.subset).exists_finset_coe
+  rw [← hI.card, ncard_coe_Finset, ← FinsetRankMatroid.matroid_indep_iff.1 hI.indep]
+  refine (M.r_mono (by simpa using hI.subset)).antisymm <| le_of_not_lt fun hlt ↦ ?_
+  obtain ⟨e, heX, heI, hr⟩ := M.indep_aug' (by simpa using hI.indep) hlt
+  have hi : M.matroid.Indep (insert e I) := by
+    rwa [← Finset.coe_insert, FinsetRankMatroid.matroid_indep_iff]
+  exact heI <| by simpa using hI.mem_of_insert_indep (e := e) (by simpa) hi
+
+@[simp] protected lemma matroid_er_eq (X : Finset α) : M.matroid.er X = M.r X := by
+  rw [← Matroid.coe_r_eq_er_of_finite _ (by simp), FinsetRankMatroid.matroid_r_eq]
+
+protected lemma matroid_er_eq_sup (X : Set α) :
+    M.matroid.er X = ⨆ Y ∈ {Y : Finset α | (Y : Set α) ⊆ X}, (M.r Y : ℕ∞) := by
+  refine le_antisymm ?_ ?_
+  set S := {Y : Finset α | (Y : Set α) ⊆ X}
+  · obtain ⟨I, hI⟩ := M.matroid.exists_basis' X
+    have aux : ∀ (J : Finset α), (J : Set α) ⊆ I → J.card ≤ ⨆ Y ∈ S, (M.r Y : ℕ∞) := by
+      intro J hJI
+      convert le_biSup (f := fun X ↦ (M.r X : ℕ∞)) (show J ∈ S from hJI.trans hI.subset) using 2
+      simpa [Eq.comm] using hI.indep.subset hJI
+    obtain (hIfin | hIinf) := I.finite_or_infinite
+    · obtain ⟨I, rfl⟩ := hIfin.exists_finset_coe
+      rw [← hI.er, FinsetRankMatroid.matroid_er_eq]
+      exact le_biSup (f := fun X ↦ (M.r X : ℕ∞)) hI.subset
+    suffices h : ⨆ Y ∈ S, (M.r Y : ℕ∞) = ⊤ by rw [h]; apply le_top
+    rw [ENat.eq_top_iff_forall_le]
+    intro b
+    obtain ⟨J, hJI, rfl⟩ := hIinf.exists_subset_card_eq b
+    rw [← FinsetRankMatroid.matroid_indep_iff.1 (hI.indep.subset hJI)]
+    apply le_biSup _ (show J ∈ S from hJI.trans hI.subset)
+  simp only [mem_setOf_eq, ← FinsetRankMatroid.matroid_er_eq, iSup_le_iff]
+  refine fun Y hYX ↦ M.matroid.er_mono hYX
+
+end FinsetRankMatroid
+
+end FinsetRank
